src/program_proof/tulip/paxos/res_network.v
@@ -1,3 +1,4 @@
+From Perennial.base_logic Require Import ghost_map.
 From Perennial.program_proof Require Import grove_prelude.
 From Perennial.program_proof.tulip.paxos Require Import base.
 
@@ -6,26 +7,47 @@ Section res_network.
   (* TODO: remove this once we have real defintions for resources. *)
   Implicit Type (γ : paxos_names).
 
-  Definition own_terminals γ (ts : gset chan) : iProp Σ.
-  Admitted.
+  Definition is_terminal γ (t : chan) : iProp Σ :=
+    ghost_map_elem γ.(trmlm) t DfracDiscarded tt.
 
-  Definition is_terminal γ (t : chan) : iProp Σ.
-  Admitted.
+  Definition own_terminals_auth γ (ts : gset chan) : iProp Σ :=
+    ghost_map_auth γ.(trmlm) 1 (gset_to_gmap tt ts).
+
+  Definition own_terminals γ (ts : gset chan) : iProp Σ :=
+    own_terminals_auth γ ts ∗ [∗ set] t ∈ ts, is_terminal γ t.
 
   #[global]
   Instance is_terminal_persistent γ t :
     Persistent (is_terminal γ t).
-  Admitted.
+  Proof. apply _. Defined.
 
   Lemma terminal_update {γ ts} t :
     own_terminals γ ts ==∗
     own_terminals γ ({[t]} ∪ ts) ∗ is_terminal γ t.
-  Admitted.
+  Proof.
+    iIntros "[Hauth #Hfrags]".
+    destruct (decide (t ∈ ts)) as [Hin | Hnotin].
+    { iDestruct (big_sepS_elem_of with "Hfrags") as "Hfrag".
+      { apply Hin. }
+      replace (_ ∪ _) with ts by set_solver.
+      by iFrame "∗ #".
+    }
+    iMod (ghost_map_insert t tt with "Hauth") as "[Hauth Hfrag]".
+    { by rewrite lookup_gset_to_gmap_None. }
+    rewrite -gset_to_gmap_union_singleton.
+    iMod (ghost_map_elem_persist with "Hfrag") as "#Hfrag".
+    iFrame "∗ #".
+    by iApply big_sepS_insert_2.
+  Qed.
 
   Lemma terminal_lookup γ ts t :
     is_terminal γ t -∗
     own_terminals γ ts -∗
     ⌜t ∈ ts⌝.
-  Admitted.
+  Proof.
+    iIntros "Hfrag [Hauth _]".
+    iDestruct (ghost_map_lookup with "Hauth Hfrag") as %Hlookup.
+    by apply lookup_gset_to_gmap_Some in Hlookup as [? _].
+  Qed.
 
 End res_network.
